proof/crypto_stream/chacha20/ref/ChaCha20_ref_proof.ec
@@ -1,6 +1,8 @@
 require import List Jasmin_model Int IntDiv IntExtra CoreMap.
 import IterOp.
 require import ChaCha20_Spec ChaCha20_ref.
+require import Array3 Array8 Array16.
+require import WArray64.
 
 lemma line_diff a b d s st i:
   i <> a => i <> d => (line a b d s st).[i] = st.[i].
@@ -8,7 +10,7 @@ proof.
   by move=> ha hd; rewrite /line /= !Array16.get_set_if ha hd /=.
 qed.
 
-lemma line_morph a b d s (st1 st2:W32.t Array16.t) i:
+lemma line_morph a b d s (st1 st2: state) i:
   i = a || i = d => 
   st1.[a] = st2.[a] => st1.[b] = st2.[b] => st1.[d] = st2.[d] =>
   (line a b d s st1).[i] = (line a b d s st2).[i].
@@ -23,7 +25,7 @@ proof.
   by move=> ha hb hc hd; rewrite /quarter_round /(\oo) !line_diff.
 qed.
 
-lemma quarter_round_morph a b c d (st1 st2:W32.t Array16.t) i:
+lemma quarter_round_morph a b c d (st1 st2:state) i:
   i = a || i = b || i = c || i = d => 
   a <> b => a <> c => a <> d =>
   b <> c => b <> d => c <> d =>
@@ -34,7 +36,7 @@ proof.
   smt (line_morph line_diff).
 qed.
 
-op column_round'  : state -> W32.t Array16.t =
+op column_round'  : state -> state  =
   quarter_round 0 4 8 12 \oo quarter_round 2 6 10 14 \oo 
   quarter_round 1 5 9 13 \oo  quarter_round 3 7 11 15.
 
@@ -45,7 +47,7 @@ proof.
   apply Array16.ext_eq => i hi_bound; smt (quarter_round_morph quarter_round_diff). 
 qed.
 
-op diagonal_round' : state -> W32.t Array16.t =
+op diagonal_round' : state -> state =
   quarter_round 1 6 11 12 \oo quarter_round 0 5 10 15 \oo quarter_round 2 7 8 13 \oo quarter_round 3 4 9 14.
 
 lemma diagonal_round'_spec st: diagonal_round st = diagonal_round' st.
@@ -55,38 +57,29 @@ proof.
   apply Array16.ext_eq => i hi_bound; smt (quarter_round_morph quarter_round_diff). 
 qed.
 
-hoare copy_state_spec (st0: WArray64.t) : M.copy_state : 
+hoare copy_state_spec st0: M.copy_state : 
   st = st0 
   ==> res = st0.
 proof. by proc; auto. qed.
 
-op is_state (st0:W32.t Array16.t) (k:WArray64.t) = 
-  st0 = Array16.init (fun i => WArray64.get32 k i).
-(*  forall i, 0 <= i < 16 => st0.[i] = . *)
-
-hoare line_spec (st0:W32.t Array16.t) a0 b0 c0 r0 : M.line : 
-  is_state st0 k /\ (a,b,c,r) = (a0,b0,c0,r0) /\ 
+hoare line_spec (st0:state) a0 b0 c0 r0 : M.line : 
+  k = st0 /\ (a,b,c,r) = (a0,b0,c0,r0) /\ 
   0 <= a0 < 16 /\ 0 <= b0 < 16 /\ 0 <= c0 < 16 /\ 
   a0 <> c0 /\ 0 <= r0 <= 16 
   ==>
-  is_state (line a0 b0 c0 r0 st0) res.
+  res = line a0 b0 c0 r0 st0.
 proof.
-  proc;auto => /> &m his h0a ha h0b hb h0c hc; rewrite eq_sym => hac h0r hr. 
-  have ? : 4 * (c{m} + 1) <= 64 by smt().
-  have ? : 4 * (a{m} + 1) <= 64 by smt().
-  rewrite /is_state his;apply Array16.ext_eq => i hi.
-  rewrite /line /= !Array16.get_set_if !Array16.initiE //.
-  rewrite !WArray64.get_set32E // h0a ha hac /= h0c hc /=.
-  case: (i=c{m}) => //=.
-  by rewrite x86_ROL_32_E /= pmod_small 1:/# .
+  proc;auto => /> &m h0a ha h0b hb h0c hc;rewrite eq_sym => hac h0r hr. 
+  apply Array16.ext_eq => i hi.
+  rewrite /line /= !Array16.get_set_if /= x86_ROL_32_E /= pmod_small /#.
 qed.
 
-hoare quarter_round_spec (st0:W32.t Array16.t) a0 b0 c0 d0 : M.quarter_round : 
-  is_state st0 k /\ (a,b,c,d) = (a0,b0,c0,d0) /\ 
+hoare quarter_round_spec (st0:state) a0 b0 c0 d0 : M.quarter_round : 
+  k = st0 /\ (a,b,c,d) = (a0,b0,c0,d0) /\ 
   a0 <> d0 /\ c0 <> b0 /\ 
   0 <= a0 < 16 /\ 0 <= b0 < 16 /\ 0 <= c0 < 16 /\ 0 <= d0 < 16
   ==>
-  is_state (quarter_round a0 b0 c0 d0 st0) res.
+  res = quarter_round a0 b0 c0 d0 st0.
 proof.
   proc => /=.
   ecall (line_spec (line a0 b0 d0 8 (line c0 d0 b0 12 (line a0 b0 d0 16 st0))) c0 d0 b0 7).
@@ -95,11 +88,11 @@ proof.
   ecall (line_spec st0 a0 b0 d0 16); auto.
 qed.
 
-hoare column_round_spec (st0:W32.t Array16.t) : M.column_round : 
-  is_state st0 k ==> is_state (column_round st0) res.
+hoare column_round_spec (st0:state) : M.column_round : 
+  k = st0 ==> res = column_round st0.
 proof.
-  conseq (_: is_state (column_round' st0) res).
-  + rewrite /is_state => &m _ r <-;apply column_round'_spec.
+  conseq (_: res = column_round' st0).
+  + by move=> &m _ r ->; rewrite column_round'_spec.
   proc; delta column_round' (\oo) => /=.
   ecall (quarter_round_spec (quarter_round 1 5 9 13 
              (quarter_round 2 6 10 14 (quarter_round 0 4 8 12 st0))) 3 7 11 15).
@@ -108,11 +101,11 @@ proof.
   ecall (quarter_round_spec st0 0 4 8 12);auto.
 qed.
 
-hoare diagonal_round_spec (st0:W32.t Array16.t) : M.diagonal_round : 
-  is_state st0 k ==> is_state (diagonal_round st0) res.
+hoare diagonal_round_spec (st0:state) : M.diagonal_round : 
+  k = st0 ==> res = diagonal_round st0.
 proof.
-  conseq (_: is_state (diagonal_round' st0) res).
-  + by rewrite /is_state => &m _ r <-; apply diagonal_round'_spec.
+  conseq (_: res = diagonal_round' st0).
+  + by move=> &m _ r ->; rewrite diagonal_round'_spec.
   proc; delta diagonal_round' (\oo) => /=.
   ecall (quarter_round_spec (quarter_round 2 7 8 13 (quarter_round 0 5 10 15 
                             (quarter_round 1 6 11 12 st0))) 3 4 9 14).
@@ -121,21 +114,21 @@ proof.
   ecall (quarter_round_spec st0 1 6 11 12);auto.
 qed.
 
-hoare round_spec (st0:W32.t Array16.t) : M.round : 
-  is_state st0 k ==> is_state (double_round st0) res.
+hoare round_spec (st0:state) : M.round : 
+  k = st0 ==> res = double_round st0.
 proof.
   proc.
   ecall (diagonal_round_spec (column_round st0)).
   by ecall (column_round_spec st0);skip;delta double_round (\oo).
 qed.
 
-hoare rounds_spec (st0: W32.t Array16.t) : M.rounds :
-  is_state st0 k ==> is_state (rounds st0) res.
+hoare rounds_spec (st0:state) : M.rounds :
+  k = st0 ==> res = rounds st0.
 proof.
   proc.
-  while (W32.to_uint c <= 10 /\ is_state (iter (W32.to_uint c) double_round st0) k).
+  while (W32.to_uint c <= 10 /\ k = iter (W32.to_uint c) double_round st0).
   + wp; ecall (round_spec (iter (to_uint c) double_round st0)); skip => />.
-    move=> &m hc hst;rewrite W32.ultE /= => hc10 r hr.
+    move=> &m hc; rewrite W32.ultE /= => hc10.
     have [h0c _] := W32.to_uint_cmp c{m}.
     have -> : to_uint (c{m} + W32.one) = W32.to_uint c{m} + 1.
     + by rewrite W32.to_uintD pmod_small //= /#.
@@ -144,13 +137,13 @@ proof.
   by rewrite W32.ultE /= /rounds /#.
 qed.
 
-
 op loads_8 (mem : global_mem_t) (from : W64.t) (len: int) = 
   map (fun i => loadW8 mem (from + W64.of_int i)) (iota_ 0 len).
 
 op loads_32 (mem: global_mem_t) (from : W64.t) (len : int) = 
   map (fun i => loadW32 mem (from + W64.of_int (4 * i))) (iota_ 0 len).
 
+(*
 lemma storesE m (a1 a2:W64.t) (l:W8.t list) :
    W64.to_uint a1 + size l <= W64.modulus =>
    loadW8 (stores m a1 l) a2 = 
@@ -165,7 +158,7 @@ proof.
      if to_uint a1 <= to_uint a2 < to_uint a1 + p then 
        l.[to_uint a2 - to_uint a1] 
      else loadW8 m a2.
- elim /natind => /=.
+  elim /natind => /=.
   + by move=> n hn0 _; rewrite iota0 1:// /#.
   move=> p hp hrec hp1.
   rewrite iotaSr 1:// -cats1 foldl_cat /= get_setE.
@@ -185,7 +178,7 @@ lemma loadW8_storeW32 m (a1 a2:W64.t) w:
        w \bits8 (W64.to_uint a2 - W64.to_uint a1)
      else loadW8 m a2.
 proof. move=> ha1;rewrite storeW32E storesE 1:// /= /#. qed.
-
+*)
 lemma loads_8D m p (n1 n2:int) : 0 <= n1 => 0 <= n2 =>
   loads_8 m p (n1 + n2) = 
   loads_8 m p n1 ++ loads_8 m (p + W64.of_int n1) n2.
@@ -220,45 +213,76 @@ proof. by rewrite /loads_8 size_map size_iota. qed.
 lemma to_uint_eq (x y:W64.t) :  (x = y) <=> (to_uint x = to_uint y).
 proof. by rewrite Core.inj_eq // (Core.can_inj _ _  W64.to_uintK). qed.
 
+lemma size_bytes_of_block st : size (bytes_of_block st) = 64.
+proof. by rewrite /bytes_of_block WArray64.size_to_list. qed.
+
+lemma map2C (f: 'a -> 'a -> 'b) (l1 l2:'a list) : 
+  (forall a1 a2, f a1 a2 = f a2 a1) =>
+  map2 f l1 l2 = map2 f l2 l1.
+proof.
+  move=> hf; elim: l1 l2=> [ | a1 l1 hrec] [ | a2 l2] //=.
+  by rewrite hf hrec.
+qed.
+
+lemma map2_take1 (f: 'a -> 'b -> 'c) (l1: 'a list) (l2: 'b list) :
+  map2 f l1 l2 = map2 f (take (size l2) l1) l2. 
+proof.
+  elim: l1 l2 => [ | a1 l1 hrec] [ | a2 l2] //=.
+  smt (size_ge0).
+qed.
+
+lemma map2_take2 (f: 'a -> 'b -> 'c) (l1: 'a list) (l2: 'b list) :
+  map2 f l1 l2 = map2 f l1 (take (size l1) l2).
+proof.
+  elim: l1 l2 => [ | a1 l1 hrec] [ | a2 l2] //=.
+  smt (size_ge0).
+qed.
+
 hoare store_spec output0 plain0 len0 k0 mem0 : M.store :
-  output = output0 /\ plain = plain0 /\ len = len0 /\ k = k0 /\ Glob.mem = mem0 /\
-  W64.to_uint output0 + 64 < W64.modulus /\
-  W64.to_uint plain0 + 64 < W64.modulus /\
-  (to_uint plain + 64 < to_uint output || to_uint output <= to_uint plain)
+  output = output0 /\ plain = plain0 /\ to_uint len = len0 /\ k = k0 /\ Glob.mem = mem0 /\ 0 <= len0 /\
+  W64.to_uint output0 + min 64 len0 < W64.modulus /\
+  W64.to_uint plain0 + min 64 len0 < W64.modulus /\
+  (to_uint plain + min 64 len0  < to_uint output || to_uint output <= to_uint plain)
   ==>
-  loads_8 Glob.mem output0 64 = map2 W8.(+^) (WArray64.to_list k0) (loads_8 mem0 plain0 64) /\
-  (forall i, 0 <= i < W64.modulus => !(to_uint output0 <= i < to_uint output0 + 64) => 
+  loads_8 Glob.mem output0 (min 64 len0) = map2 W8.(+^) (bytes_of_block k0) (loads_8 mem0 plain0 (min 64 len0)) /\
+  (forall i, 0 <= i < W64.modulus => !(to_uint output0 <= i < to_uint output0 + (min 64 len0)) => 
      loadW8 Glob.mem (W64.of_int i) = loadW8 mem0 (W64.of_int i)) /\
-  res.`1 = output0 + W64.of_int 64 /\
-  res.`2 = plain0 + W64.of_int 64 /\
-  res.`3 = len0 - W32.of_int 64.
+  res.`1 = output0 + W64.of_int (min 64 len0) /\
+  res.`2 = plain0 + W64.of_int (min 64 len0) /\
+  res.`3 = W32.of_int len0 - W32.of_int (min 64 len0).
 proof.
   proc; inline *; wp => /=.
-  while (0 <= i <= 64 /\
-         output = output0 /\ plain = plain0 /\ k0 = k /\ 
-         W64.to_uint output0 + 64 < W64.modulus /\
-         W64.to_uint plain0 + 64 < W64.modulus /\
-         (to_uint plain + 64 < to_uint output || to_uint output <= to_uint plain) /\
+  pose len1 := min 64 len0.
+  while (0 <= i <= len1 /\
+         output = output0 /\ plain = plain0 /\ k0 = k /\ len = W32.of_int len0 /\ 0 <= len0 /\
+         W64.to_uint output0 + len1 < W64.modulus /\
+         W64.to_uint plain0 + len1 < W64.modulus /\
+         (to_uint plain + len1 < to_uint output || to_uint output <= to_uint plain) /\
          loads_8 Glob.mem output0 i = 
-           map2 W8.(+^) 
-             (map (fun i => WArray64."_.[_]" k0 i) (iota_ 0 i))
+           map2 W8.(+^) (take i (bytes_of_block k0))
+(*             (map (fun i => WArray64."_.[_]" k0 i) (iota_ 0 i)) *)
              (loads_8 mem0 plain0 i) /\
          (forall j, 0 <= j < W64.modulus => !(to_uint output0 <= j < to_uint output0 + i) => 
             loadW8 Glob.mem (W64.of_int j) = loadW8 mem0 (W64.of_int j))).
-  + wp; skip => /> &m h0i _ hob hpb hdisj hloads hdiff hi16;split; 1:smt().
+  + wp; skip => /> &m h0i _ hlen0 hob hpb hdisj hloads hdiff + hi64.
+    have ismall : to_uint (W32.of_int i{m}) = i{m}.
+    + by rewrite W32.to_uint_small 1:/#.
+    rewrite W32.ultE ismall => hilen.
+    split; 1:smt().
     have hpi : to_uint (plain{m} + W64.of_int i{m}) = to_uint plain{m} + i{m}.
     + by rewrite  W64.to_uintD_small W64.to_uint_small /#.
     have hoi : to_uint (output{m} + W64.of_int i{m}) = to_uint output{m} + i{m}.
     + by rewrite  W64.to_uintD_small W64.to_uint_small /#. 
     split.
-    + rewrite !loads_8D // iota_add // map_cat map2_cat.
-      + by rewrite size_map size_iota size_loads_8.
+    + rewrite !loads_8D // (take_nth W8.zero) 1:size_bytes_of_block 1:// -cats1 map2_cat. 
+      + rewrite size_take // size_bytes_of_block hi64 size_loads_8 /#.
       congr.
       + rewrite -hloads;apply loads_8_eq; 1:smt().
         move=> j hj.        
         rewrite  /loadW8 storeW8E get_set_neqE_s //.
         by rewrite to_uint_eq W64.to_uint_small; smt (W64.to_uint_cmp). 
-      rewrite /loads_8 /= /loadW8 storeW8E /=;congr => //.
+      rewrite /loads_8 /= /loadW8 storeW8E /=;congr.
+      + by rewrite /bytes_of_block -WArray64.get_to_list.
       rewrite (hdiff (to_uint (plain{m} + W64.of_int i{m}))).
       + by rewrite hpi; smt (W64.to_uint_cmp).
       + by rewrite hpi /#.
@@ -266,44 +290,53 @@ proof.
     move=> j h0j hjb hj.
     rewrite -hdiff 1:// 1:/# /loadW8 storeW8E get_set_neqE_s //.
     by rewrite to_uint_eq W64.to_uint_small 1:// hoi /#.
-  wp;skip => /> *;split.
-  + by rewrite /loads_8 iota0.
-  move=> mem i0 h1 h2 h3.
-  have ->> -> /> : i0 = 64 by smt(). 
-  by move=> h *;apply h.
+  wp;skip => &hr /> *. 
+  split; 1:split.
+  + smt().
+  + by rewrite /loads_8 iota0 // take0.
+  move=> mem i0; rewrite W32.ultE => + h2 h3.
+  have ismall : to_uint (W32.of_int i0) = i0.
+  + by rewrite W32.to_uint_small 1:/#.
+  rewrite ismall => h1 /=.
+  have ->> /> ??? -> hdiff: i0 = len1 by smt(). 
+  split.
+  + have {1}-> : len1 = size (loads_8 Glob.mem{hr} plain{hr} len1).
+    + by rewrite size_loads_8 /#.
+    by rewrite -map2_take1.
+  split; 1: by move=> *;apply hdiff.
+  by rewrite W32.of_intS /=.
 qed.
 
 hoare sum_states_spec k0 st0 : M.sum_states : 
-  is_state k0 k /\ is_state st0 st
+  k = k0 /\ st = st0
   ==>
-  is_state (Array16.map2 (fun (x y: W32.t) => x + y) k0 st0) res.
+  res = Array16.map2 (fun (x y: W32.t) => x + y) k0 st0.
 proof.
   proc.
   rewrite /is_state. 
   unroll for 2;wp;skip => /> &hr.
   by apply Array16.all_eq_eq;rewrite /all_eq.
 qed.
-  
-lemma init16_set12 t w : 
-  Array16.init (WArray64.get32 (WArray64.set32 t 12 w)) = 
-  (Array16.init (WArray64.get32 t)).[12 <- w].
-proof. by apply Array16.all_eq_eq;rewrite /Array16.all_eq /=. qed.
+
+lemma take_loads_8 mem p (n1 n2:int) : n1 <= n2 =>
+  take n1 (loads_8 mem p n2) = loads_8 mem p n1.
+proof. by move=> hn;rewrite /loads_8 -map_take take_iota /#. qed.
 
 hoare chacha20_ref_spec output0 plain0 key0 nonce0 counter0 : M.chacha20_ref :
-   output = output0 /\ 
-   (to_uint plain{hr} + W32.to_uint len < to_uint output{hr} || to_uint output{hr} <= to_uint plain{hr}) /\
-   to_uint output{hr} + to_uint len < W64.modulus /\
-   to_uint plain{hr} + to_uint len < W64.modulus /\
-   plain0 = loads_8 Glob.mem plain (W32.to_uint len) /\
-   key0 = Array8.of_list W32.zero (loads_32 Glob.mem key 8) /\
-   nonce0 = Array3.of_list W32.zero (loads_32 Glob.mem nonce 3) /\
-   counter0 = counter 
-   ==> 
-   (chacha20_CTR_encrypt_bytes key0 nonce0 counter0 plain0).`1 = 
-   loads_8 Glob.mem output0 (size plain0).
+  output = output0 /\ 
+  (to_uint plain{hr} + W32.to_uint len < to_uint output{hr} || to_uint output{hr} <= to_uint plain{hr}) /\
+  to_uint output{hr} + to_uint len < W64.modulus /\
+  to_uint plain{hr} + to_uint len < W64.modulus /\
+  plain0 = loads_8 Glob.mem plain (W32.to_uint len) /\
+  key0 = Array8.of_list W32.zero (loads_32 Glob.mem key 8) /\
+  nonce0 = Array3.of_list W32.zero (loads_32 Glob.mem nonce 3) /\
+  counter0 = counter 
+  ==> 
+  (chacha20_CTR_encrypt_bytes key0 nonce0 counter0 plain0).`1 = 
+  loads_8 Glob.mem output0 (size plain0).
 proof.
   proc; rewrite /chacha20_CTR_encrypt_bytes /=.
-  seq 3: 
+  seq 1: 
     ((to_uint plain{hr} + W32.to_uint len < to_uint output{hr} || to_uint output{hr} <= to_uint plain{hr}) /\
     to_uint output{hr} + to_uint len < W64.modulus /\
     to_uint plain{hr} + to_uint len < W64.modulus /\
@@ -312,186 +345,99 @@ proof.
       let splain1 = size plain1 in
       to_uint output0 = to_uint output{hr} - size plain1 /\
       plain0 = plain1 ++ loads_8 Glob.mem plain ilen /\
-      is_state (setup key0 nonce0 c) st /\
-      iter (splain1 %/ 64) (ctr_round key0 nonce0) ([], plain0, counter0) = 
+      st = setup key0 nonce0 c /\
+      (0 < ilen => splain1 %% 64 = 0) /\
+      iter (splain1 %/ 64 + b2i (splain1 %% 64 <> 0) ) (ctr_round key0 nonce0) ([], plain0, counter0) = 
          (loads_8 Glob.mem output0 splain1, loads_8 Glob.mem plain ilen, c)).
-  + conseq />;inline M.init.
-    unroll for 15; unroll for 12; wp; skip => &m /> ???.
+  + inline M.init.
+    unroll for 12; unroll for 9; wp; skip => &m /> ???.
     exists [] counter{m} => /=.
-    rewrite /is_state;split; 2: by rewrite /= div0z iter0.
+    rewrite iter0 // /loads_8 /=.
     rewrite /setup /loads_32 /=.
     rewrite Array8.of_listK 1:// Array3.of_listK 1:// /=.
-    pose l1 := (c0::_). pose l2 := (Array16.init _).
-    (* why did we need the pose l1, l2 ? *)
-    apply: (Core.canLR _ _ l1 l2 (Array16.to_listK witness)).
-    by rewrite /l1 /l2 /c0 /c1 /c2 /c3 /Array16.to_list /mkseq.
-  seq 1 : (#pre).
+    split;2: done.
+    by apply Array16.all_eq_eq; rewrite /Array16.all_eq.
   + while (#pre) => //.
     elim * => plain1 counter1 /=.
     inline M.increment_counter; wp.
     pose st0 := (setup key0 nonce0 counter1).
-    ecall (store_spec output plain len k Glob.mem).
+    ecall (store_spec output plain (W32.to_uint len) k Glob.mem); last first.
+    + move=> &hr /> ???? h result mem h1 h2 h3 h4 h5. 
+      apply (h result mem _). 
+      by rewrite h1 /= h3 h4 h5 W32.of_intS /= => *;apply h2.
     ecall (sum_states_spec (rounds st0) st0).
     ecall (rounds_spec st0).
     ecall (copy_state_spec st).
-    skip => /> &hr hnot hout hplain hout0 hst hiter ^ hule.
-    have h64 : to_uint (W32.of_int 64) = 64 by rewrite W32.to_uint_small.
-    have h64' : to_uint (W64.of_int 64) = 64 by rewrite W64.to_uint_small.
-    rewrite W32.uleE h64 => hlen hst0 res0 hres0 res1 hres1.
+    skip => /> &hr hnot hout hplain hout0 hmod hiter. 
+    rewrite W32.ultE /= => hult.
+    pose len1 := min 64 (to_uint len{hr}). 
+    have hlen1 : to_uint (W32.of_int len1) = len1 by rewrite W32.to_uint_small /#.
+    have hlen1' : to_uint (W64.of_int len1) = len1 by rewrite W64.to_uint_small /#.
+    split; 1: smt().
+    move=> hlen ho64 hp64 hop [output' plain' len'] mem hload hdiff /= 3!->>.
+    rewrite W32.to_uintB. 
+    + by rewrite W32.uleE hlen1 /#.
+    rewrite !W64.to_uintD_small hlen1' //.
     split; 1:smt().
-    move=> ho64 hp64 hop [output' plain' len'] mem hload hdiff /= 3!->>.
-    rewrite W32.to_uintB 1:// h64.
-    rewrite !W64.to_uintD_small h64' //;split; 1:smt().
     split;[smt() | split;1:smt()].
-    exists (plain1 ++ loads_8 Glob.mem{hr} plain{hr} 64) (counter1 + W32.of_int 1).
+    exists (plain1 ++ loads_8 Glob.mem{hr} plain{hr} len1) (counter1 + W32.of_int 1).
     split. 
     + by rewrite size_cat size_loads_8 /#.  
     split.
     + rewrite -catA; congr.
-      have -> : loads_8 mem (plain{hr} + W64.of_int 64) (to_uint len{hr} - 64) = 
-                loads_8 Glob.mem{hr} (plain{hr} + W64.of_int 64) (to_uint len{hr} - 64).
+      rewrite hlen1.     
+      have -> : loads_8 mem (plain{hr} + W64.of_int len1) (to_uint len{hr} - len1) = 
+                loads_8 Glob.mem{hr} (plain{hr} + W64.of_int len1) (to_uint len{hr} - len1).
       + apply loads_8_eq. 
-        + by rewrite W64.to_uintD_small h64' // /#.
-        by move=> i; rewrite W64.to_uintD_small h64' 1://; smt (W64.to_uint_cmp).
+        + by rewrite W64.to_uintD_small hlen1' // /#.
+        by move=> i; rewrite W64.to_uintD_small hlen1' 1://; smt (W64.to_uint_cmp).
       by rewrite -loads_8D 1:// /#. 
     split.
-    + move: hst; rewrite /setup /is_state init16_set12 => hst.
-      rewrite -hst -!catA;apply Array16.all_eq_eq;rewrite /Array16.all_eq /=.
-      rewrite !nth_cat; rewrite Array8.size_to_list /=.
-      have -> : WArray64.get32 st{hr} 12 = (Array16.init (WArray64.get32 st{hr})).[12] by done.
-      by rewrite -hst /= -catA nth_cat Array8.size_to_list.
-    rewrite size_cat size_loads_8 /max /= -{1}(mul1z 64) divzMDr 1:// addzC iterS.
-    + by apply divz_ge0 => //; apply List.size_ge0.
+    + rewrite /setup /=; apply Array16.all_eq_eq. 
+      rewrite -!catA /Array16.all_eq /=.
+      by rewrite !nth_cat; rewrite Array8.size_to_list /=.
+    split.
+    + rewrite hlen1 size_cat size_loads_8 /max => h.
+      have -> /= : len1 = 64 by smt().
+      rewrite modzDr;apply hmod => /#.
+    pose plain2 := plain1 ++ loads_8 Glob.mem{hr} plain{hr} len1.
+    have -> : size plain2 %/ 64 + b2i (size plain2 %% 64 <> 0) = 
+              ((size plain1 %/ 64 + b2i (size plain1 %% 64 <> 0))) + 1.
+    + rewrite /plain2 size_cat size_loads_8 (_ : max 0 len1 = len1) 1:/# hmod 1:// /b2i /=.
+      have ?: 64 %| size plain1 by rewrite /(%|) hmod. 
+      rewrite dvdz_modzDl 1:// divzDl 1://.
+      case: (64 <= to_uint len{hr}) => hlt.
+      + smt (modzz divzz).
+      smt (divz_small modz_small W32.to_uint_cmp). 
+    rewrite iterS. 
+    + smt (modz_ge0 divz_ge0 size_ge0).
     rewrite hiter /ctr_round /=;split.
-    + rewrite loads_8D 1:List.size_ge0 1://;congr.
-      apply loads_8_eq;1:by rewrite hout0 /#.
-      move=> i hi;rewrite hdiff 3://; smt (W64.to_uint_cmp).
-    have -> : output0 + W64.of_int (size plain1) = output{hr}.
-    + have hplain1 : to_uint (W64.of_int (size plain1)) = size plain1.
-      + rewrite W64.to_uint_small; smt (W64.to_uint_cmp size_ge0).
-      by apply to_uint_eq; rewrite W64.to_uintD_small hplain1 /#. 
-    rewrite hload.
-rewrite /bytes_of_block /chacha20_block hst /= /chacha20_core.
-
- hst0.
-print is_state.
-smt().
-W64.to_uintD_small. admit.
-;  smt().
-      have := W64.to_uintK.
-      
-
-admit.
-    admit.
-   
-print ge0_size.
-
-search (0 <= _ %/ _).
-search iter.
-iterS
-search Int.(+) (%/).
-((_ + _) %% _).
-      done. 
-ext_eq => x hx.
-      rewrite Array16.get_setE 1://;case: (x=12) => [->> | hne].
-      + rewrite -catA /= nth_cat Array8.size_to_list /=.
-        admit.
-
-      search nth.
-Array8.size
-search nth (++).
-all_eq_eq; apply Array
-
-rewrite /Array16.all_eq. 
-print Array16.allP.
- apply Array16.allP.
-
-print
-rewrite /Array16.all_eq /=.
-
-(init ((get32 ((set32 st{hr} 12 ((get32 st{hr} 12)%WArray64 + W32.one)))%WArray64))%WArray64)%Array16
-1:/#.
-
-search W64.to_uint W64.(+).
-    have : to_uint (len{hr} - (of_int 64)%W32) = to_uint len{hr} - 64.
-W32.to_uintB
-search W32.to_uint W32.([-]).
-
- split. smt(). split. smt(). smt().
-search W64.to_uint W64.of_int.
- W64.to_uint_small.
-search W32.(\ule).
-    to_uint output{hr} + to_uint len < W64.modulus.
-    to_uint plain{hr} + to_uint len < W64.modulus.
-print rounds_spec.
-    
-
-
-
- proc store (output:W64.t, plain:W64.t, len:W32.t, k:WArray64.t) : W64.t *
-                                                                    W64.t *
-                                                                    W32.t = {
-    var aux: int;
-    
-    var i:int;
-    
-    i <- 0;
-    while (i < 16) {
-      k = set32 k i ((get32 k i) `^` (loadW32 Glob.mem (plain + (W64.of_int (4 * i)))));
-      Glob.mem <-
-      storeW32 Glob.mem (output + (W64.of_int (4 * i))) (get32 k i);
-      i <- i + 1;
-    }
-    (output, plain, len) <@ update_ptr (output, plain, len, 64);
-    return (output, plain, len);
-  }
-  
-    print ctr_round.
-print c0.
-search Array16.of_list.
-
-    rewrite /all_eq => />.
-search Array8.to_list Array8.of_list.
- /all_eq => />.
-
-   (iter (if ilen %% 64 = 0 then ilen %/ 64 else ilen %/ 64 + 1) 
-     (ctr_round key0 nonce0)
-     (loads_8 Glob.mem output0 (size plain1), loads_8 Glob.mem ilen, get32 st 12)) 
-print ctr_round.
-
-is_state (setup key0 nonce0 counter) st.
-
-
-search IterOp.iter Int.(+).
-
-  seq 3 : 
-
- proc init (key:W64.t, nonce:W64.t, counter:W32.t) : WArray64.t = {
-    var aux: int;
-    
-    var st:WArray64.t;
-    var i:int;
-    st <- WArray64.create W8.zero;
-    st = set32 st 0 (W32.of_int 1634760805);
-    st = set32 st 1 (W32.of_int 857760878);
-    st = set32 st 2 (W32.of_int 2036477234);
-    st = set32 st 3 (W32.of_int 1797285236);
-    i <- 0;
-    while (i < 8) {
-      st = set32 st (4 + i) (loadW32 Glob.mem (key + (W64.of_int (4 * i))));
-      i <- i + 1;
-    }
-    st = set32 st 12 counter;
-    i <- 0;
-    while (i < 3) {
-      st = set32 st (13 + i) (loadW32 Glob.mem (nonce + (W64.of_int (4 * i))));
-      i <- i + 1;
-    }
-    return (st);
-  }
-
-  proc chacha20_ref (output:W64.t, plain:W64.t, len:W32.t, key:W64.t,
-                     nonce:W64.t, counter:W32.t) : unit = {
-
-proc chacha20_ref (output:W64.t, plain:W64.t, len:W32.t, key:W64.t,
-                     nonce:W64.t, counter:W32.t)
+    + rewrite /plain2 size_cat size_loads_8 /max (_: 0 < len1) 1:/# /=.
+      rewrite loads_8D 1:size_ge0 1:/#;congr.
+      + apply loads_8_eq;1:by rewrite hout0 /#.
+        by move=> i hi;rewrite hdiff 3://; smt (W64.to_uint_cmp).
+      have -> : output0 + W64.of_int (size plain1) = output{hr}.
+      + have hplain1 : to_uint (W64.of_int (size plain1)) = size plain1.
+        + rewrite W64.to_uint_small; smt (W64.to_uint_cmp size_ge0).
+        by apply to_uint_eq; rewrite W64.to_uintD_small hplain1 /#. 
+      rewrite hload /chacha20_block /chacha20_core /=.
+      rewrite map2C; 1:by apply W8.xorwC.
+      case : (to_uint len{hr} < 64) => hlt; 1:smt().
+      have -> : len1 = 64 by smt().
+      by rewrite map2_take2 size_bytes_of_block take_loads_8 1:/#.
+    case : (64 < to_uint len{hr}) => hlt;last first.
+    + by rewrite drop_oversize 1:size_loads_8 1:/# /len1 /min hlt /= /loads_8.
+    have {1} -> : to_uint len{hr} = len1 + (to_uint len{hr} - len1) by ring.
+    rewrite loads_8D 1,2:/#.
+    have -> : len1 = 64 by rewrite /len1 /min hlt.
+    rewrite drop_size_cat 1:size_loads_8 1:// /=.
+    have h : to_uint (plain{hr} + W64.of_int 64) + (to_uint len{hr} - 64) = to_uint plain{hr} + to_uint len{hr}. 
+    + by rewrite W64.to_uintD_small /= 1:/#; ring.
+    apply loads_8_eq; smt(W64.to_uint_cmp).
+  skip => &hr /> h1 h2 h3 plain1 c ??? mem len0 output1 plain2.
+  rewrite W32.ultE /= => hlen0.
+  have -> /= : to_uint len0 = 0 by smt (W32.to_uint_cmp).
+  move=> ??? plain3 c2 h4.
+  have -> : loads_8 mem plain2 0 = [] by rewrite /loads_8.
+  by rewrite cats0 => -> ->.
+qed.
