proof/crypto_stream/chacha20/ref/Array8.ec
@@ -1,0 +1,3 @@
+require import Jasmin_array.
+
+clone export PolyArray as Array8  with op size <- 8.
